% Auto-converted from khan-exercises
\documentclass{article}
\usepackage{amsmath,amssymb}
\usepackage[T1]{fontenc}
\usepackage{textcomp}
\newcommand{\abs}[1]{\lvert #1\rvert}

\begin{document}
\section*{Hyperbola and ellipse intuition}
\textbf{Question.} The equation of a north-south opening hyperbola is :
                        \textbackslash\{\}qquad $\frac{(x - x_1)^2}{b^2}$ - $\frac{(y - y_1)^2}{a^2}$ = 1.
                    
                    
                        Find the foci of the hyperbola below by moving the orange points to their correct positions.
                        Then use that information to find the values of y\_1, x\_1, a and b.

\textbf{Answer.} [graph.focus1.coord, graph.focus2.coord]
                        
                            if (\_.isEqual(guess, [[-2, 2], [2, 2]])) \{
                                return "";
                            \}

                            return guess[0][0] === H \&\& guess[1][0] === H \&\&
                                (guess[0][1] === K - C \&\& guess[1][1] === K + C) ||
                                (guess[0][1] === K + C \&\& guess[1][1] === K - C)
                        
                        
                            graph.focus1.setCoord(guess[0]);
                            graph.focus2.setCoord(guess[1]);
                        
                    

                    
                        Equation of the hyperbola:
                        
                            
                                y\_1 = 
                                [[K]]
                            
                            
                                x\_1 = 
                                [[H]]
                            
                            
                                a = 
                                [[A]]
                            
                            
                                b = 
                                [[B]]

\textbf{Hints.}
\begin{itemize}
  \item For all points on a hyperbola, the absolute value of the distance from one focus minus the distance to the other focus is equal.
                        There is only one way to arrange the two foci such that this is true.
                        Show me
  \item One focus is ([[H]], [[K + C]]) and the other is ([[H]], [[K - C]]).
  \item x\_1 and y\_1 are the coordinates of the center of the hyperbola.
  \item The center of a hyperbola is at the midpoint of its two foci.
                        \textbackslash\{\}left($\frac{[[H]] + [[H]]}{2}$, $\frac{[[K+C]] + [[K-C]]}{2}$\textbackslash\{\}right) = ([[H]], [[K]])
  \item The absolute value of the distance from one focus minus the distance to the other focus is equal to 2a
  \item \textbackslash\{\}qquad\textbackslash\{\}begin\{align*\}
                            2a \&= [[2 * A]] \textbackslash\{\}\textbackslash\{\}
                            a \&= [[A]]\textbackslash\{\}end\{align*\}
  \item The focal distance, c is the distance between the center of the hyperbola to either focus.
                        \textbackslash\{\}qquad\textbackslash\{\}begin\{align*\}
                            c\textasciicircum{}2 \&= a\textasciicircum{}2 + b\textasciicircum{}2 \textbackslash\{\}\textbackslash\{\}
                            b\textasciicircum{}2 \&= c\textasciicircum{}2 - a\textasciicircum{}2 \textbackslash\{\}\textbackslash\{\}
                            b \&= $\sqrt{c^2 - a^2}$ \textbackslash\{\}\textbackslash\{\}
                            b \&= $\sqrt{[[C]]^2 - [[A]]^2}$ \textbackslash\{\}\textbackslash\{\}
                            b \&= $\sqrt{[[C * C - A * A]]}$ \textbackslash\{\}\textbackslash\{\}
                            b \&= [[B]]\textbackslash\{\}end\{align*\}
  \item So the equation of the hyperbola is
                        $\frac{(y - [[K]])^2}{[[A]]^2}$ - $\frac{(x - [[H]])^2}{[[B]]^2}$ = 1.
  \item For all points on a hyperbola, the absolute value of the distance from one focus minus the distance to the other focus is equal.
                        There is only one way to arrange the two foci such that this is true.
                        Show me
  \item One focus is ([[K - C]], [[H]]) and the other is ([[K + C]], [[H]]).
  \item x\_1 and y\_1 are the coordinates of the center of the hyperbola.
  \item The center of a hyperbola is at the midpoint of its two foci.
                        \textbackslash\{\}left($\frac{[[K - C]] + [[K + C]]}{2}$, $\frac{[[H]] + [[H]]}{2}$\textbackslash\{\}right) = ([[K]], [[H]])
  \item The absolute value of the distance from one focus minus the distance to the other focus is equal to 2a
  \item \textbackslash\{\}qquad\textbackslash\{\}begin\{align*\}
                            2a \&= [[2 * A]] \textbackslash\{\}\textbackslash\{\}
                            a \&= [[A]]\textbackslash\{\}end\{align*\}
  \item The focal distance, c is the distance between the center of the hyperbola to either focus.
                        \textbackslash\{\}qquad\textbackslash\{\}begin\{align*\}
                            c\textasciicircum{}2 \&= a\textasciicircum{}2 + b\textasciicircum{}2 \textbackslash\{\}\textbackslash\{\}
                            b\textasciicircum{}2 \&= c\textasciicircum{}2 - a\textasciicircum{}2 \textbackslash\{\}\textbackslash\{\}
                            b \&= $\sqrt{c^2 - a^2}$ \textbackslash\{\}\textbackslash\{\}
                            b \&= $\sqrt{[[C]]^2 - [[A]]^2}$ \textbackslash\{\}\textbackslash\{\}
                            b \&= $\sqrt{[[C * C - A * A]]}$ \textbackslash\{\}\textbackslash\{\}
                            b \&= [[B]]\textbackslash\{\}end\{align*\}
  \item So the equation of the hyperbola is
                        $\frac{(x - [[H]])^2}{[[B]]^2}$ + $\frac{(y - [[K]])^2}{[[A]]^2}$ = 1.
\end{itemize}
\end{document}
