% Auto-converted from khan-exercises
\documentclass{article}
\usepackage{amsmath,amssymb}
\usepackage[T1]{fontenc}
\usepackage{textcomp}
\newcommand{\abs}[1]{\lvert #1\rvert}

\begin{document}
\section*{Equations with variables on both sides}
\textbf{Question.} Solve for x:

\textbf{Answer.} x = [[( D - B ) / ( A - C )]]

\textbf{Hints.}
\begin{itemize}
  \item Subtract [[C]]x from both sides:
                    ([[A]]x + [[B]]) - [[C]]x = ([[C]]x + [[D]]) - [[C]]x
                    [[A - C]]x + [[B]] = [[D]]
                
                
                    Subtract [[abs(B)]] from both sides:Add [[abs(B)]] to both sides:
                    ([[A - C]]x + [[B]]) + [[-B]] = [[D]] + [[-B]]
                    [[A - C]]x = [[D - B]]
                
                
                    Divide both sides by [[A - C]].
                    $\frac{[[A - C]]x}{[[A - C]]}$ = $\frac{[[D - B]]}{[[A - C]]}$
                
                
                    Simplify.
                    x = [[SOLUTION]]
  \item Subtract [[A]]x from both sides:
                    ([[A]]x + [[B]]) - [[A]]x = ([[C]]x + [[D]]) - [[A]]x
                    [[B]] = [[C - A]]x + [[D]]
                
                
                    Subtract [[abs(D)]] from both sides:Add [[abs(D)]] to both sides:
                    [[B]] + [[-D]] = ([[C - A]]x + [[D]]) + [[-D]]
                    [[B - D]] = [[C - A]]x
                
                
                    Divide both sides by [[C - A]].
                    $\frac{[[B - D]]}{[[C - A]]}$ = $\frac{[[C - A]]x}{[[C - A]]}$
                
                
                    Simplify.
                    [[SOLUTION]] = x
\end{itemize}
\end{document}
